theories/Typing.v
@@ -54,6 +54,7 @@ Inductive Typed : context -> term -> type -> Prop :=
       Typed G' e s ->
       Typed G e s
   | TLet : forall G D x e e' s t Gxs GD,
+      Inert e ->
       ~fv G x ->
       Typed D e s ->
       Fill G (CtxHasTy x s) Gxs ->
